iris_heap_lang/lib/rw_lock.v
@@ -1,0 +1,65 @@
+From iris.base_logic.lib Require Export invariants.
+From iris.bi.lib Require Export fractional.
+From iris.heap_lang Require Import primitive_laws notation.
+From iris.prelude Require Import options.
+
+(** A general interface for a reader-writer lock.
+
+All parameters are implicit, since it is expected that there is only one
+[heapGS_gen] in scope that could possibly apply.
+
+Only one instance of this class should ever be in scope. To write a library that
+is generic over the lock, just add a [`{rwlock}] implicit parameter. To use a
+particular lock instance, use [Local Existing Instance <rwlock instance>].
+
+When writing an instance of this class, please take care not to shadow the class
+projections (e.g., either use [Local Definition newlock] or avoid the name
+ [newlock] altogether), and do not register an instance -- just make it a
+[Definition] that others can register later. *)
+Class rwlock `{!heapGS_gen hlc Σ} := RwLock {
+  (** * Operations *)
+  newlock : val;
+  acquire_reader : val;
+  release_reader : val;
+  acquire_writer : val;
+  release_writer : val;
+  (** * Predicates *)
+  (** [lock_name] is used to associate [reader_locked] and [writer_locked] with
+  [is_rw_lock] *)
+  lock_name : Type;
+  (** No namespace [N] parameter because we only expose program specs, which
+  anyway have the full mask. *)
+  is_rw_lock (γ : lock_name) (lock : val) (Φ : Qp → iProp Σ) : iProp Σ;
+  reader_locked (γ : lock_name) (q : Qp) : iProp Σ;
+  writer_locked (γ : lock_name) : iProp Σ;
+  (** * General properties of the predicates *)
+  is_rw_lock_persistent γ lk Φ :> Persistent (is_rw_lock γ lk Φ);
+  is_rw_lock_iff γ lk Φ Ψ :
+    is_rw_lock γ lk Φ -∗ ▷ □ (∀ q,  Φ q ↔ Ψ q) -∗ is_rw_lock γ lk Ψ;
+  reader_locked_timeless γ q :> Timeless (reader_locked γ q);
+  writer_locked_timeless γ :> Timeless (writer_locked γ);
+  writer_locked_exclusive γ : writer_locked γ -∗ writer_locked γ -∗ False;
+  (** * Program specs *)
+  newlock_spec (Φ : Qp → iProp Σ) `{!AsFractional P Φ 1} :
+    {{{ P }}}
+      newlock #()
+    {{{ lk γ, RET lk; is_rw_lock γ lk Φ }}};
+  acquire_reader_spec γ lk Φ :
+    {{{ is_rw_lock γ lk Φ }}}
+      acquire_reader lk
+    {{{ q, RET #(); reader_locked γ q ∗ Φ q }}};
+  release_reader_spec γ lk Φ q :
+    {{{ is_rw_lock γ lk Φ ∗ reader_locked γ q ∗ Φ q }}}
+      release_reader lk
+    {{{ RET #(); True }}};
+  acquire_writer_spec γ lk Φ :
+    {{{ is_rw_lock γ lk Φ }}}
+      acquire_writer lk
+    {{{ RET #(); writer_locked γ ∗ Φ 1%Qp }}};
+  release_writer_spec γ lk Φ :
+    {{{ is_rw_lock γ lk Φ ∗ writer_locked γ ∗ Φ 1%Qp }}}
+      release_writer lk
+    {{{ RET #(); True }}};
+}.
+Global Hint Mode rwlock + + + : typeclass_instances.
+
